merge with tlb

pageTable.dfy
@@ -17,7 +17,7 @@ class PageTable{
   const offset := 12
   const pageSize: addr := 0x0FFF
   const numVpns: addr := 0x0010_0000
-  const numOffsets := 0x1000
+  const numOffsets: addr := 0x1000
   const numVpnParts: addr := 0x0400
   var currPfn: addr
 
@@ -25,8 +25,9 @@ class PageTable{
   reads this
   reads root
   reads tlbValid, tlbKeys, tlbVals
-  {0 <= currPfn < numVpns &&
-  root.Length == numVpns as int &&
+reads if (root.Length == numVpnParts as int) then set i | 0 <= i < numVpnParts && root[i].Some? :: root[i].arr else {}
+  {0 < currPfn < numVpns &&
+  root.Length == numVpnParts as int &&
   // TLB arrays are well-formed
   tlbKeys.Length == tlbSize &&
   tlbVals.Length == tlbSize &&
@@ -35,7 +36,11 @@ class PageTable{
   // when valid, TLB entries carry valid vpn/pfn ranges
   (forall i: nat :: 0 <= i < tlbSize as int ==> (tlbValid[i] ==> (tlbKeys[i] < numVpns && tlbVals[i] < numVpns))) &&
   // all pageTables have exactly `numVpns` entries
-  forall i : nat :: ((0 <= i < root.Length) ==> (root[i] == Nil || root[i].arr.Length == numVpnParts as int))
+  (forall i : nat :: ((0 <= i < root.Length) ==> (root[i] == Nil || root[i].arr.Length == numVpnParts as int))) &&
+
+// all pageTables have exactly `numVpns` entries
+(forall i : nat :: ((0 <= i < root.Length) ==> (root[i] == Nil || root[i].arr.Length == numVpnParts as int))) &&
+(currPfn != 0 ==> (forall i : nat :: ((0 <= i < root.Length && root[i].Some?) ==> (forall j : nat :: (0 <= j < root[i].arr.Length) ==> root[i].arr[j] < currPfn))))
 
   }
 
@@ -45,23 +50,21 @@ class PageTable{
   ensures forall j: nat :: 0 <= j < tlbSize ==> tlbValid[j] == false
   {
 
-    root := new secondLevelPtr[numVpns];
+  root := new secondLevelPtr[numVpnParts];
 
     new;
 
-    assert(root.Length == numVpns as int);
-    for i := 0 to numVpns as int
-      invariant root.Length == numVpns as int
-      invariant 0 <= i <= root.Length
-      invariant forall j: nat :: 0 <= j < i ==> root[j] == Nil
-      invariant fresh(root){
-      root[i] := Nil by {
-        assert(root.Length == numVpns as int);
+  assert(root.Length == numVpnParts as int);
+  for i := 0 to numVpnParts as int
+    invariant root.Length == numVpnParts as int
+    invariant 0 <= i <= root.Length
+    invariant forall j: nat :: 0 <= j < i ==> root[j] == Nil
+    invariant fresh(root){
+    root[i] := Nil by {
+      assert(root.Length == numVpnParts as int);
 
       }
     }
-    currPfn := 1;
-    assert(currPfn == 1 as addr);
     assert(!root[0].Some?);
     // initialize TLB
     tlbKeys := new addr[tlbSize];
@@ -78,14 +81,73 @@ class PageTable{
     assert forall j: nat :: 0 <= j < tlbSize ==> !tlbValid[j];
     //assert(forall i : nat :: ((0 <= i < root.Length) ==> (root[i] == Nil)));
     // completely null
+    currPfn := 1;
+    assert(currPfn == 1 as addr);
 
   }
   /*lemma insertThenGet(vpnPart1: addr, vpnPart2: addr, pfn: addr)
   requires 0 <= vpnPart1 < numVpnParts
   requires 0 <= vpnPart2 < numVpnParts{
     var err := tryInsertMapping(vpnPart1, vpnPart2, pfn);
+=======
+}*/
+lemma bvLess(a: nat, b: nat)
+requires 0 <= a <= 0xFFFF_FFFF
+requires 0 <= b <= 0xFFFF_FFFF
+requires a < b
+//ensures a as bv32 < b as bv32
+{
+}
 
-  }*/
+lemma bvLessAddr(a: addr, b: addr)
+requires 0 <= a <= 0xFFFF_FFFF
+requires 0 <= b <= 0xFFFF_FFFF
+requires a < b
+//ensures a as bv32 < b as bv32
+{
+  var aNat := a as nat;
+  var bNat := b as nat;
+  //assert(aNat as bv32 < bNat as bv32) by {
+    //bvLess(aNat, bNat);
+  //}
+}
+
+method buildAddr(pfn: addr, offset: addr) 
+returns (a: addr)
+requires 0 <= pfn < numVpns
+requires 0 <= offset < numOffsets
+//ensures (a as bv32 & 0xFFF) == offset as bv32
+//ensures (a as bv32 >> 12) == pfn as bv32
+{
+  var mask1: bv32 := 0xF_FFFF;
+  var b1 := (pfn as bv32 & mask1);
+  //assert(b1 == pfn as bv32);
+  assert(b1 <= mask1);
+  //assert(b1 < 0x1 as bv32 << 20);
+  //assert(b1 <= 0xF_FFFF as bv32);
+
+  //assert(pfnBv < numVpns as bv32);
+  //assert(0x10_0000 == 1 as bv32 << 20 as bv6);
+  //assert(pfnBv < numVpns as bv21);
+  var shifted := (b1 << 12);
+  //assert(shifted >> 12 == b1);
+  //assert(shifted >> 32 == 0);
+  //assert(shifted >> 12 == pfnBv) by {
+  //}
+  //assert(shifted & 0xFFF == 0);
+  var b := (shifted | offset as bv32);
+  
+  //assert(b >> 12 == pfnBv) by {
+    //assert(offset as bv32 >> 12 == 0) by {
+      //assert(0 <= offset < 0xFFF);
+      //assert(0xFFF as bv32 == )
+  //}
+  //assert(b & 0x0FFF == offset as bv32);
+  return (b as addr);
+}
+function getOffset(a: addr): addr {
+  (a as bv32 & 0x0FFF as bv32) as addr
+}
 
   method getVpn(vaddr: addr) returns(vpn: addr)
   ensures 0 <= vpn < numVpns{
@@ -116,64 +178,93 @@ class PageTable{
     assert(b2 <= 0x03FF as bv32);
     part1 := b1 as addr;    
     part2 := b2 as addr;    
+
   }
 
-  // internal functions
-  method tryInsertMapping(vpnPart1: addr, vpnPart2: addr, pfn: addr) returns (err: nat)
-  requires pageTableInvariant()
+// internal functions
+method tryInsertMapping(vpnPart1: addr, vpnPart2: addr, pfn: addr) returns (err: nat)
+requires pageTableInvariant()
+requires 0 <= vpnPart1 < numVpnParts
+requires 0 <= vpnPart2 < numVpnParts
+requires pfn < currPfn
+ensures 0 <= err <= 1
+ensures pageTableInvariant()
+ensures err == 0 ==> root[vpnPart1].Some? && root[vpnPart1].arr[vpnPart2] == pfn
+ensures (err != 0 && old(root[vpnPart1].Some?)) ==> root[vpnPart1].Some? && root[vpnPart1].arr == old(root[vpnPart1].arr)
+modifies root
+modifies if root[vpnPart1].Some? then {root[vpnPart1].arr} else {}
+{
+assert(forall i : nat :: ((0 <= i < root.Length) ==> (root[i] == Nil || root[i].arr.Length == numVpnParts as int)));
+assert(forall i : nat :: ((0 <= i < root.Length && root[i].Some?) ==> (forall j :: (0 <= j < root[i].arr.Length) ==> root[i].arr[j] < currPfn)));
+
+  var entry1 := root[vpnPart1];
+
+  if (entry1 == Nil){
+assert(forall i : nat :: ((0 <= i < root.Length) ==> (root[i] == Nil || root[i].arr.Length == numVpnParts as int)));
+    var a := new addr[numVpnParts];
+    for i := 0 to numVpnParts as int
+      invariant a.Length == numVpnParts as int
+      invariant 0 <= i <= a.Length
+      invariant forall j: nat :: 0 <= j < i ==> a[j] == 0 as addr
+      // these invariants are irrelevant to this loop but are necessary to prove later assertions
+      invariant forall i : nat :: ((0 <= i < root.Length) ==> (root[i] == Nil || root[i].arr.Length == numVpnParts as int))
+      invariant forall i : nat :: ((0 <= i < root.Length && root[i].Some?) ==> (forall j :: (0 <= j < root[i].arr.Length) ==> root[i].arr[j] < currPfn))
+      {
+      a[i] := 0 as addr by {
+        assert(a.Length == numVpnParts as int);
+
+      }
+    }
+    assert(forall i :: 0 <= i < a.Length ==> a[i] == 0 as addr);
+
+    entry1 := Some(a);
+    root[vpnPart1] := entry1;
+    assert(entry1.arr.Length == numVpnParts as int);
+  }
+
+
+  assert entry1.Some?;
+
+  var entry2: addr := entry1.arr[vpnPart2] by {
+    assert(forall i : nat :: ((0 <= i < root.Length) ==> (root[i] == Nil || root[i].arr.Length == numVpnParts as int)));
+    assert(0 <= vpnPart2 < numVpnParts);
+  }
+  
+  if (entry2 == 0){
+    entry2 := pfn;
+    entry1.arr[vpnPart2] := entry2;
+    assert(entry2 < currPfn);
+  }
+  
+
+  if (entry2 == pfn){
+    // important assertions
+    var getPfn := tryGetMapping(vpnPart1, vpnPart2) by {
+      assert(forall i : nat :: ((0 <= i < root.Length) ==> (root[i] == Nil || root[i].arr.Length == numVpnParts as int))) ;
+      assert(forall j :: 0 <= j < numVpnParts ==> root[vpnPart1].arr[j] < currPfn) by {
+        assert(root[vpnPart1].Some? && root[vpnPart1].arr[vpnPart2] == pfn);
+        assert(old(root[vpnPart1].Some?) ==> forall j :: 0 <= j < numVpnParts && j != vpnPart2 ==> root[vpnPart1].arr[j] == old(root[vpnPart1].arr[j]));
+        assert(old(root[vpnPart1].Some?) ==> forall j :: 0 <= j < numVpnParts && j != vpnPart2 ==> root[vpnPart1].arr[j] < currPfn);
+        assert(!old(root[vpnPart1].Some?) ==> forall j :: 0 <= j < numVpnParts && j != vpnPart2 ==> root[vpnPart1].arr[j] == 0);
+      }
+      assert(forall i : nat :: ((0 <= i < root.Length && root[i].Some?) ==> (forall j :: (0 <= j < root[i].arr.Length) ==> root[i].arr[j] < currPfn)));
+    }
+    assert(pfn == getPfn);
+    return 0;
+  } else{
+    // vaddr is alr in use
+    // TODO use a free entry
+    return 1;
+  }
+}
+method tryGetMapping(vpnPart1: addr, vpnPart2: addr) returns (pfn: addr)
   requires 0 <= vpnPart1 < numVpnParts
   requires 0 <= vpnPart2 < numVpnParts
-  ensures 0 <= err <= 1
-  ensures pageTableInvariant()
-  ensures err == 0 ==> root[vpnPart1].Some? && root[vpnPart1].arr[vpnPart2] == pfn
-  modifies root
-  modifies if root[vpnPart1].Some? then {root[vpnPart1].arr} else {}
-  {
-  assert(forall i : nat :: ((0 <= i < root.Length) ==> (root[i] == Nil || root[i].arr.Length == numVpnParts as int)));
-
-    var entry1 := root[vpnPart1];
-
-    if (entry1 == Nil){
-      var a := new addr[numVpnParts];
-      entry1 := Some(a);
-      root[vpnPart1] := entry1;
-      assert(entry1.arr.Length == numVpnParts as int);
-      entry1.arr[0] := 1;
-    }
-
-
-    assert entry1.Some?;
-
-    var entry2: addr := entry1.arr[vpnPart2] by {
-      assert(forall i : nat :: ((0 <= i < root.Length) ==> (root[i] == Nil || root[i].arr.Length == numVpnParts as int)));
-      assert(0 <= vpnPart2 < numVpnParts);
-    }
-    
-    if (entry2 == 0){
-      entry2 := pfn;
-      entry1.arr[vpnPart2] := entry2;
-    }
-    
-
-    if (entry2 == pfn){
-      // important assertions
-      var getPfn := tryGetMapping(vpnPart1, vpnPart2);
-      assert(pfn == getPfn);
-      return 0;
-    } else{
-      // vaddr is alr in use
-      // TODO use a free entry
-      return 1;
-    }
-  }
-
-  method tryGetMapping(vpnPart1: addr, vpnPart2: addr) returns (pfn: addr)
-    requires 0 <= vpnPart1 < numVpnParts
-    requires 0 <= vpnPart2 < numVpnParts
-    requires pageTableInvariant()
-  ensures pageTableInvariant()
-  ensures root[vpnPart1].Some? ==> pfn == root[vpnPart1].arr[vpnPart2]
-  {
+  requires pageTableInvariant()
+ensures pageTableInvariant()
+ensures root[vpnPart1].Some? ==> pfn == root[vpnPart1].arr[vpnPart2]
+ensures currPfn != 0 ==> 0 <= pfn < currPfn
+{
 
     var entry1 := root[vpnPart1];
 
@@ -185,11 +276,6 @@ class PageTable{
     var entry2 := entry1.arr[vpnPart2];
     
     return entry2;
-  }
-
-  method getPfn(vpn: addr) returns (pfn: addr)
-  requires false{
-    //pfn := tryGetMapping(vpn);
   }
 
 
@@ -275,6 +361,9 @@ class PageTable{
   method translate(vaddr: addr) returns (paddr: addr, ok: bool)
     requires pageTableInvariant()
     ensures pageTableInvariant()
+modifies root
+modifies set i | 0 <= i < numVpnParts && root[i].Some? :: root[i].arr
+modifies this
   {
     var vpn := getVpn(vaddr);
     var pfn, hit := tlbLookup(vpn);
@@ -287,21 +376,27 @@ class PageTable{
     }
 
     var part1, part2 := maskVpn(vpn);
+    currPfn := currPfn + 1;
     pfn := tryGetMapping(part1, part2);
-    if (pfn == 0) {
-      paddr := 0;
-      ok := false;
-      return;
+    if (pfn == 0){
+      var err := allocate(vaddr, 1);
+      if (err != 0) {
+        paddr := 0;
+        ok := false;
+        return;
+      }
+
     }
     // insert into TLB on a miss
     tlbInsert(vpn, pfn);
-    var offBits2 := (vaddr as bv32 & pageSize as bv32);
-    var phys2 := ((pfn as bv32) << offset) | offBits2;
-    paddr := phys2 as addr;
+    var offset := getOffset(vaddr);
+
+    paddr := buildAddr(pfn, offset);
+
     ok := true;
   }
-
 }
+
 
 /*method main(){
   var pt := new PageTable();
